adequacy tmp

theories/iris_adequacy.v
@@ -26,6 +26,12 @@ Let reducible := @reducible wasm_lang.
 
 Context `{!wfuncG Σ, !wtabG Σ, !wmemG Σ, !wmemsizeG Σ, !wglobG Σ, !wframeG Σ}.
 
+(*
+   t and Φs should be a list of expr and iProp each; for each pair in t and Φ,
+   we have WP e {{ Φ }}.
+
+   Why is this definition useful, though?
+*)
 Notation wptp s t Φs := ([∗ list] e;Φ ∈ t;Φs, WP e @ s; ⊤ {{ Φ }})%I.
 
 (* Given that (e1, σ1) -> (e2, σ2) with 'effects' efs, plus the state interp
@@ -54,6 +60,7 @@ Proof.
   by iFrame.
 Qed.
 
+(* Seems similar to above, but uses step instead of prim_step. *)
 Lemma wptp_step s es1 es2 κ κs σ1 ns σ2 Φs nt :
   step (es1,σ1) κ (es2, σ2) →
   state_interp σ1 ns (κ ++ κs) nt -∗ wptp s es1 Φs -∗
@@ -65,9 +72,23 @@ Proof.
   destruct Hstep as [e1' σ1' e2' σ2' efs t2' t3 Hstep]; simplify_eq/=.
   iDestruct (big_sepL2_app_inv_l with "Ht") as (Φs1 Φs2 ->) "[? Ht]".
   iDestruct (big_sepL2_cons_inv_l with "Ht") as (Φ Φs3 ->) "[Ht ?]".
-  iExists _. iMod (wp_step with "Hσ Ht") as "H"; first done. iModIntro.
-  iApply (step_fupdN_wand with "H"). iIntros ">($ & He2 & Hefs) !>".
+  iExists (length efs). iMod (wp_step with "Hσ Ht") as "H"; first by [].
+  (* TODO: these are bad patterns -- they exist because our state_interp does
+     not use the ns, nt or observations, so these variables cannot be
+     instantiated automatically. *)
+  instantiate (1 := 0).
+  instantiate (1 := []).
+  instantiate (1 := 0).
+  iModIntro.
+  iApply (step_fupdN_wand with "H").
+  iIntros "H".
+  iMod "H" as "($ & H)".
+  iDestruct "H" as (f) "(Hframe & He2 & Hefs)".
+  iModIntro.
   rewrite -(assoc_L app) -app_comm_cons. iFrame.
+  (* TODO: We can actually prove a stronger result here. Check if this makes
+     sense. *)
+  by iApply "He2".
 Qed.
 
 (* The total number of laters used between the physical steps number
@@ -79,6 +100,210 @@ Local Fixpoint steps_sum (num_laters_per_step : nat → nat) (start ns : nat) : 
     S $ num_laters_per_step start + steps_sum num_laters_per_step (S start) ns
   end.
 
+Let nsteps := @iris.program_logic.language.nsteps wasm_lang.
+
+Lemma wptp_steps s n es1 es2 κs κs' σ1 σ2 Φs ns nt :
+  nsteps n (es1, σ1) κs (es2, σ2) →
+  state_interp σ1 ns (κs ++ κs') nt -∗ wptp s es1 Φs
+  ={⊤}[∅]▷=∗^n ∃ nt',
+    state_interp σ2 (n+ns) κs' (nt + nt') ∗ wptp s es2 (Φs ++ replicate nt' fork_post).
+Proof.
+  revert nt es1 es2 κs κs' σ1 σ2 Φs.
+  induction n as [|n IH]=> nt es1 es2 κs κs' σ1 σ2 Φs /=.
+  { inversion_clear 1; iIntros "? ?"; iExists 0=> /=.
+    rewrite right_id_L. by iFrame. }
+  iIntros (Hsteps) "Hσ He". inversion_clear Hsteps as [|?? [t1' σ1']].
+  iDestruct (wptp_step with "Hσ He") as (nt') ">H"; first eauto; simplify_eq.
+  iMod "H".
+  iIntros "!> !>". iMod "H". iMod "H" as "(Hσ & He)". iModIntro.
+  iApply (step_fupdN_wand with "[Hσ He]"); first by iApply (IH with "Hσ He").
+  iDestruct 1 as (nt'') "[??]".
+  rewrite -(assoc_L app) -replicate_plus.
+  by eauto with iFrame.
+  Unshelve. exact [].
+  Unshelve. exact 0.
+  Unshelve. exact 0.
+  Unshelve. exact 0.
+  Unshelve. exact [].
+Qed.
+
+Lemma wp_not_stuck κs ns nt e σ Φ :
+  state_interp ns σ κs nt -∗ WP e {{ Φ }} ={⊤}=∗ ⌜not_stuck e σ⌝.
+Proof.
+  rewrite wp_unfold /wp_pre /not_stuck. iIntros "Hσ H".
+  destruct (to_val e) as [v|] eqn:?; first by eauto.
+  iSpecialize ("H" $! σ [] κs with "Hσ"). rewrite sep_elim_l.
+  iMod (fupd_plain_mask with "H") as %?; eauto.
+Qed.
+
+Lemma wptp_strong_adequacy Φs κs' s n es1 es2 κs σ1 σ2 nt:
+  nsteps n (es1, σ1) κs (es2, σ2) →
+  state_interp σ1 (κs ++ κs') nt -∗
+  wptp s es1 Φs ={⊤}[∅]▷=∗^(S n) ∃ nt',
+    ⌜ ∀ e2, s = NotStuck → e2 ∈ es2 → not_stuck e2 σ2 ⌝ ∗
+    state_interp σ2 κs' (nt + nt') ∗
+    [∗ list] e;Φ ∈ es2;Φs ++ replicate nt' fork_post, from_option Φ True (to_val e).
+Proof.
+  iIntros (Hstep) "Hσ He". rewrite Nat_iter_S_r.
+  iDestruct (wptp_steps with "Hσ He") as "Hwp"; first done.
+  iApply (step_fupdN_wand with "Hwp").
+  iDestruct 1 as (nt') "(Hσ & Ht)"; simplify_eq/=.
+  iMod (fupd_plain_keep_l ⊤
+    ⌜ ∀ e2, s = NotStuck → e2 ∈ es2 → not_stuck e2 σ2 ⌝%I
+    (state_interp σ2 κs' (nt + nt') ∗ wptp s es2 (Φs ++ replicate nt' fork_post))%I
+    with "[$Hσ $Ht]") as "(%&Hσ&Hwp)".
+  { iIntros "(Hσ & Ht)" (e' -> He').
+    move: He' => /(elem_of_list_split _ _)[?[?->]].
+    iDestruct (big_sepL2_app_inv_l with "Ht") as (Φs1 Φs2 ?) "[? Hwp]".
+    iDestruct (big_sepL2_cons_inv_l with "Hwp") as (Φ Φs3 ->) "[Hwp ?]".
+    iMod (wp_not_stuck with "Hσ Hwp") as "$"; auto. }
+  iApply step_fupd_fupd. iApply step_fupd_intro; first done. iNext.
+  iExists _. iSplitR; first done. iFrame "Hσ".
+  iApply big_sepL2_fupd.
+  iApply (big_sepL2_impl with "Hwp").
+  iIntros "!#" (? e Φ ??) "Hwp".
+  destruct (to_val e) as [v2|] eqn:He2'; last done.
+  apply of_to_val in He2' as <-. simpl. iApply wp_value_fupd'. done.
+Qed.
+End adequacy.
+
+(** Iris's generic adequacy result *)
+Theorem wp_strong_adequacy Σ Λ `{!invPreG Σ} es σ1 n κs t2 σ2 φ :
+  (∀ `{Hinv : !invG Σ},
+    ⊢ |={⊤}=> ∃
+         (s: stuckness)
+         (stateI : state Λ → list (observation Λ) → nat → iProp Σ)
+         (Φs : list (val Λ → iProp Σ))
+         (fork_post : val Λ → iProp Σ),
+       let _ : irisG Λ Σ := IrisG _ _ Hinv stateI fork_post in
+       stateI σ1 κs 0 ∗
+       ([∗ list] e;Φ ∈ es;Φs, WP e @ s; ⊤ {{ Φ }}) ∗
+       (∀ es' t2',
+         (* es' is the final state of the initial threads, t2' the rest *)
+         ⌜ t2 = es' ++ t2' ⌝ -∗
+         (* es' corresponds to the initial threads *)
+         ⌜ length es' = length es ⌝ -∗
+         (* If this is a stuck-free triple (i.e. [s = NotStuck]), then all
+         threads in [t2] are not stuck *)
+         ⌜ ∀ e2, s = NotStuck → e2 ∈ t2 → not_stuck e2 σ2 ⌝ -∗
+         (* The state interpretation holds for [σ2] *)
+         stateI σ2 [] (length t2') -∗
+         (* If the initial threads are done, their post-condition [Φ] holds *)
+         ([∗ list] e;Φ ∈ es';Φs, from_option Φ True (to_val e)) -∗
+         (* For all forked-off threads that are done, their postcondition
+            [fork_post] holds. *)
+         ([∗ list] v ∈ omap to_val t2', fork_post v) -∗
+         (* Under all these assumptions, and while opening all invariants, we
+         can conclude [φ] in the logic. After opening all required invariants,
+         one can use [fupd_mask_subseteq] to introduce the fancy update. *)
+         |={⊤,∅}=> ⌜ φ ⌝)) →
+  nsteps n (es, σ1) κs (t2, σ2) →
+  (* Then we can conclude [φ] at the meta-level. *)
+  φ.
+Proof.
+  intros Hwp ?.
+  eapply (step_fupdN_soundness' _ (S (S n)))=> Hinv. rewrite Nat_iter_S.
+  iMod Hwp as (s stateI Φ fork_post) "(Hσ & Hwp & Hφ)".
+  iDestruct (big_sepL2_length with "Hwp") as %Hlen1.
+  iApply step_fupd_intro; [done|]; iModIntro.
+  iApply step_fupdN_S_fupd. iApply (step_fupdN_wand with "[-Hφ]").
+  { iApply (@wptp_strong_adequacy _ _ (IrisG _ _ Hinv stateI fork_post) _ []
+    with "[Hσ] Hwp"); eauto; by rewrite right_id_L. }
+  iDestruct 1 as (nt' ?) "(Hσ & Hval) /=".
+  iDestruct (big_sepL2_app_inv_r with "Hval") as (es' t2' ->) "[Hes' Ht2']".
+  iDestruct (big_sepL2_length with "Ht2'") as %Hlen2.
+  rewrite replicate_length in Hlen2; subst.
+  iDestruct (big_sepL2_length with "Hes'") as %Hlen3.
+  iApply fupd_plain_mask_empty.
+  iApply ("Hφ" with "[//] [%] [//] Hσ Hes'"); [congruence|].
+  by rewrite big_sepL2_replicate_r // big_sepL_omap.
+Qed.
+
+(** Since the full adequacy statement is quite a mouthful, we prove some more
+intuitive and simpler corollaries. These lemmas are morover stated in terms of
+[rtc erased_step] so one does not have to provide the trace. *)
+Record adequate {Λ} (s : stuckness) (e1 : expr Λ) (σ1 : state Λ)
+    (φ : val Λ → state Λ → Prop) := {
+  adequate_result t2 σ2 v2 :
+   rtc erased_step ([e1], σ1) (of_val v2 :: t2, σ2) → φ v2 σ2;
+  adequate_not_stuck t2 σ2 e2 :
+   s = NotStuck →
+   rtc erased_step ([e1], σ1) (t2, σ2) →
+   e2 ∈ t2 → not_stuck e2 σ2
+}.
+
+Lemma adequate_alt {Λ} s e1 σ1 (φ : val Λ → state Λ → Prop) :
+  adequate s e1 σ1 φ ↔ ∀ t2 σ2,
+    rtc erased_step ([e1], σ1) (t2, σ2) →
+      (∀ v2 t2', t2 = of_val v2 :: t2' → φ v2 σ2) ∧
+      (∀ e2, s = NotStuck → e2 ∈ t2 → not_stuck e2 σ2).
+Proof.
+  split.
+  - intros []; naive_solver.
+  - constructor; naive_solver.
+Qed.
+
+Theorem adequate_tp_safe {Λ} (e1 : expr Λ) t2 σ1 σ2 φ :
+  adequate NotStuck e1 σ1 φ →
+  rtc erased_step ([e1], σ1) (t2, σ2) →
+  Forall (λ e, is_Some (to_val e)) t2 ∨ ∃ t3 σ3, erased_step (t2, σ2) (t3, σ3).
+Proof.
+  intros Had ?.
+  destruct (decide (Forall (λ e, is_Some (to_val e)) t2)) as [|Ht2]; [by left|].
+  apply (not_Forall_Exists _), Exists_exists in Ht2; destruct Ht2 as (e2&?&He2).
+  destruct (adequate_not_stuck NotStuck e1 σ1 φ Had t2 σ2 e2) as [?|(κ&e3&σ3&efs&?)];
+    rewrite ?eq_None_not_Some; auto.
+  { exfalso. eauto. }
+  destruct (elem_of_list_split t2 e2) as (t2'&t2''&->); auto.
+  right; exists (t2' ++ e3 :: t2'' ++ efs), σ3, κ; econstructor; eauto.
+Qed.
+
+Corollary wp_adequacy Σ Λ `{!invPreG Σ} s e σ φ :
+  (∀ `{Hinv : !invG Σ} κs,
+     ⊢ |={⊤}=> ∃
+         (stateI : state Λ → list (observation Λ) → iProp Σ)
+         (fork_post : val Λ → iProp Σ),
+       let _ : irisG Λ Σ := IrisG _ _ Hinv (λ σ κs _, stateI σ κs) fork_post in
+       stateI σ κs ∗ WP e @ s; ⊤ {{ v, ⌜φ v⌝ }}) →
+  adequate s e σ (λ v _, φ v).
+Proof.
+  intros Hwp. apply adequate_alt; intros t2 σ2 [n [κs ?]]%erased_steps_nsteps.
+  eapply (wp_strong_adequacy Σ _); [|done]=> ?.
+  iMod Hwp as (stateI fork_post) "[Hσ Hwp]".
+  iExists s, (λ σ κs _, stateI σ κs), [(λ v, ⌜φ v⌝%I)], fork_post => /=.
+  iIntros "{$Hσ $Hwp} !>" (e2 t2' -> ? ?) "_ H _".
+  iApply fupd_mask_intro_discard; [done|]. iSplit; [|done].
+  iDestruct (big_sepL2_cons_inv_r with "H") as (e' ? ->) "[Hwp H]".
+  iDestruct (big_sepL2_nil_inv_r with "H") as %->.
+  iIntros (v2 t2'' [= -> <-]). by rewrite to_of_val.
+Qed.
+
+Corollary wp_invariance Σ Λ `{!invPreG Σ} s e1 σ1 t2 σ2 φ :
+  (∀ `{Hinv : !invG Σ} κs,
+     ⊢ |={⊤}=> ∃
+         (stateI : state Λ → list (observation Λ) → nat → iProp Σ)
+         (fork_post : val Λ → iProp Σ),
+       let _ : irisG Λ Σ := IrisG _ _ Hinv stateI fork_post in
+       stateI σ1 κs 0 ∗ WP e1 @ s; ⊤ {{ _, True }} ∗
+       (stateI σ2 [] (pred (length t2)) -∗ ∃ E, |={⊤,E}=> ⌜φ⌝)) →
+  rtc erased_step ([e1], σ1) (t2, σ2) →
+  φ.
+Proof.
+  intros Hwp [n [κs ?]]%erased_steps_nsteps.
+  eapply (wp_strong_adequacy Σ _); [|done]=> ?.
+  iMod (Hwp _ κs) as (stateI fork_post) "(Hσ & Hwp & Hφ)".
+  iExists s, stateI, [(λ _, True)%I], fork_post => /=.
+  iIntros "{$Hσ $Hwp} !>" (e2 t2' -> _ _) "Hσ H _ /=".
+  iDestruct (big_sepL2_cons_inv_r with "H") as (? ? ->) "[_ H]".
+  iDestruct (big_sepL2_nil_inv_r with "H") as %->.
+  iDestruct ("Hφ" with "Hσ") as (E) ">Hφ".
+  by iApply fupd_mask_intro_discard; first set_solver.
+Qed.
+
+
+
+
+(* This is wptp_step but with the single step replaced by the nsteps predicate. *)
 Lemma wptp_steps s n es1 es2 κs κs' σ1 ns σ2 Φs nt :
   nsteps n (es1, σ1) κs (es2, σ2) →
   state_interp σ1 ns (κs ++ κs') nt -∗ wptp s es1 Φs
@@ -89,11 +314,11 @@ Proof.
   revert nt es1 es2 κs κs' σ1 ns σ2 Φs.
   induction n as [|n IH]=> nt es1 es2 κs κs' σ1 ns σ2 Φs /=.
   { inversion_clear 1; iIntros "? ?"; iExists 0=> /=.
-    rewrite Nat.add_0_r right_id_L. iFrame. by iApply fupd_mask_subseteq. }
+    rewrite right_id_L. iFrame. by iApply fupd_mask_subseteq. }
   iIntros (Hsteps) "Hσ He". inversion_clear Hsteps as [|?? [t1' σ1']].
-  rewrite -(assoc_L (++)) Nat_iter_add plus_n_Sm.
   iDestruct (wptp_step with "Hσ He") as (nt') ">H"; first eauto; simplify_eq.
   iModIntro. iApply step_fupdN_S_fupd. iApply (step_fupdN_wand with "H").
+  iIntros "H".
   iIntros ">(Hσ & He)". iMod (IH with "Hσ He") as "IH"; first done. iModIntro.
   iApply (step_fupdN_wand with "IH"). iIntros ">IH".
   iDestruct "IH" as (nt'') "[??]".
